Logic/Modal/Standard/PLoN/Soundness.lean
@@ -4,30 +4,42 @@ namespace LO.Modal.Standard
 
 namespace PLoN
 
-open Formula
+open System Formula
 
 variable {p : Formula α} {Λ : DeductionParameter α}
 
-lemma sound (defines : Λ.DefinesPLoNFrameClass 𝔽) (d : Λ ⊢! p) : 𝔽 ⊧ p := by
+lemma sound (characterized : Λ.CharacterizedByPLoNFrameClass 𝔽) (d : Λ ⊢! p) : 𝔽 ⊧ p := by
   intro F hF;
-  have := defines.mpr hF;
+  have := characterized hF;
   exact Semantics.RealizeSet.setOf_iff.mp this p d;
 
-lemma sound_of_defines (defines : Λ.DefinesPLoNFrameClass 𝔽) : Sound Λ 𝔽 := ⟨sound defines⟩
+lemma sound_of_characterized (defines : Λ.CharacterizedByPLoNFrameClass 𝔽) : Sound Λ 𝔽 := ⟨sound defines⟩
 
-lemma unprovable_bot_of_nonempty_frameclass (defines : Λ.DefinesPLoNFrameClass 𝔽) (nonempty : 𝔽.Nonempty) : Λ ⊬! ⊥ := by
+lemma unprovable_bot_of_nonempty_frameclass (characterized : Λ.CharacterizedByPLoNFrameClass 𝔽) (nonempty : 𝔽.Nonempty) : Λ ⊬! ⊥ := by
   intro h;
   obtain ⟨⟨_, F⟩, hF⟩ := nonempty;
-  simpa using sound defines h hF;
+  simpa using sound characterized h hF;
 
-lemma consistent_of_defines (defines : Λ.DefinesPLoNFrameClass 𝔽) (nonempty : 𝔽.Nonempty) : System.Consistent Λ := by
+lemma consistent_of_characterized (characterized : Λ.CharacterizedByPLoNFrameClass 𝔽) (nonempty : 𝔽.Nonempty) : System.Consistent Λ := by
   apply System.Consistent.of_unprovable;
-  exact unprovable_bot_of_nonempty_frameclass defines nonempty;
+  exact unprovable_bot_of_nonempty_frameclass characterized nonempty;
 
 
-instance : Sound 𝐍 (AllFrameClass α) := sound_of_defines N_defines
+instance : Sound 𝐍 (AllFrameClass α) := sound_of_characterized N_characterized
 
-instance : System.Consistent (𝐍 : DeductionParameter α) := consistent_of_defines N_defines AllFrameClass.nonempty
+instance : Sound 𝐍𝟒 (TransitiveFrameClass α) := sound_of_characterized N4_characterized
+
+instance : Sound 𝐍(𝐑) (SerialFrameClass α) := sound_of_characterized NRosser_characterized
+
+instance : Sound 𝐍𝟒(𝐑) (TransitiveSerialFrameClass α) := sound_of_characterized N4Rosser_characterized
+
+instance : System.Consistent (𝐍 : DeductionParameter α) := consistent_of_characterized N_characterized AllFrameClass.nonempty
+
+instance : System.Consistent (𝐍𝟒 : DeductionParameter α) := consistent_of_characterized N4_characterized TransitiveFrameClass.nonempty
+
+instance : System.Consistent (𝐍(𝐑) : DeductionParameter α) := consistent_of_characterized NRosser_characterized SerialFrameClass.nonempty
+
+instance : System.Consistent (𝐍𝟒(𝐑) : DeductionParameter α) := consistent_of_characterized N4Rosser_characterized TransitiveSerialFrameClass.nonempty
 
 end PLoN
 
